vera/VerilogTypecheck.v
@@ -37,14 +37,6 @@ Definition TCContext := width.
 
 Definition TC := sum string.
 
-Equations expr_type : TypedVerilog.expression -> Verilog.vtype :=
-  expr_type (TypedVerilog.BinaryOp t _ _ _) := t;
-  expr_type (TypedVerilog.BitSelect _ _) := 0;
-  expr_type (TypedVerilog.Conditional _ tBranch fBranch) := expr_type tBranch; (**  TODO: need to check fBranch? *)
-  expr_type (TypedVerilog.Conversion _ t _) := t;
-  expr_type (TypedVerilog.IntegerLiteral v) := size v;
-  expr_type (TypedVerilog.NamedExpression t _) := t.
-
 Equations tc_lvalue : TCBindings -> Verilog.expression -> TC TypedVerilog.expression :=
   tc_lvalue Γ (Verilog.BinaryOp op l r) :=
     raise "Binary operator not permitted as lvalue"%string;
@@ -74,7 +66,7 @@ Equations tc_expr : option TCContext -> TCBindings -> Verilog.expression -> TC T
       =>
         typed_l <- tc_expr ctx Γ l ;;
         typed_r <- tc_expr ctx Γ r ;;
-        ret (TypedVerilog.BinaryOp (max (expr_type typed_l) (expr_type typed_r)) op typed_l typed_r)
+        ret (TypedVerilog.BinaryOp (max (TypedVerilog.expr_type typed_l) (TypedVerilog.expr_type typed_r)) op typed_l typed_r)
     | Verilog.BinaryShiftRight (* '>>' *)
     | Verilog.BinaryShiftLeft (* '<<' *)
     | Verilog.BinaryShiftRightArithmetic (* '>>>' *)
@@ -82,7 +74,7 @@ Equations tc_expr : option TCContext -> TCBindings -> Verilog.expression -> TC T
       =>
         typed_l <- tc_expr ctx Γ l ;;
         typed_r <- tc_expr None Γ r ;;
-        ret (TypedVerilog.BinaryOp (expr_type typed_l) op typed_l typed_r)
+        ret (TypedVerilog.BinaryOp (TypedVerilog.expr_type typed_l) op typed_l typed_r)
     | Verilog.BinaryLessThan (* '<' *)
     | Verilog.BinaryLessThanEqual (* '<=' *)
     | Verilog.BinaryGreaterThan (* '>' *)
@@ -97,13 +89,13 @@ Equations tc_expr : option TCContext -> TCBindings -> Verilog.expression -> TC T
         typed_l <- tc_expr None Γ l ;;
         typed_r <- tc_expr None Γ r ;;
         (* TODO: Make sure we are doing zero-extension here *)
-        match Nat.compare (expr_type typed_l) (expr_type typed_r) with
+        match Nat.compare (TypedVerilog.expr_type typed_l) (TypedVerilog.expr_type typed_r) with
         | Lt => 
-            typed_l_final <- tc_expr (Some (expr_type typed_r)) Γ l ;;
-            ret (TypedVerilog.BinaryOp (expr_type typed_r) op typed_l_final typed_r)
+            typed_l_final <- tc_expr (Some (TypedVerilog.expr_type typed_r)) Γ l ;;
+            ret (TypedVerilog.BinaryOp (TypedVerilog.expr_type typed_r) op typed_l_final typed_r)
         | Gt => 
-            typed_r_final <- tc_expr (Some (expr_type typed_l)) Γ r ;;
-            ret (TypedVerilog.BinaryOp (expr_type typed_l) op typed_l typed_r_final)
+            typed_r_final <- tc_expr (Some (TypedVerilog.expr_type typed_l)) Γ r ;;
+            ret (TypedVerilog.BinaryOp (TypedVerilog.expr_type typed_l) op typed_l typed_r_final)
         | Eq => ret (TypedVerilog.BinaryOp 1 op typed_l typed_r)
         end
     | Verilog.BinaryLogicalAnd (* '&&' *)
@@ -131,7 +123,7 @@ Equations tc_expr : option TCContext -> TCBindings -> Verilog.expression -> TC T
     typed_cond <- tc_expr ctx Γ cond ;;
     typed_tBranch <- tc_expr ctx Γ tBranch ;;
     typed_fBranch <- tc_expr ctx Γ fBranch ;;
-    if (eq_dec (expr_type typed_tBranch) (expr_type typed_fBranch)) then
+    if (eq_dec (TypedVerilog.expr_type typed_tBranch) (TypedVerilog.expr_type typed_fBranch)) then
       ret (TypedVerilog.Conditional typed_cond typed_tBranch typed_fBranch)
     else
       (**  TODO: Should probably upcast, *)
@@ -179,11 +171,11 @@ Equations tc_stmt : TCBindings -> Verilog.statement -> TC TypedVerilog.Statement
     TypedVerilog.Block <$> mapT (tc_stmt Γ) body;
   tc_stmt Γ (Verilog.BlockingAssign lhs rhs) :=
     typed_lhs <- tc_lvalue Γ lhs ;;
-    typed_rhs <- tc_expr (Some (expr_type typed_lhs)) Γ rhs ;;
+    typed_rhs <- tc_expr (Some (TypedVerilog.expr_type typed_lhs)) Γ rhs ;;
     ret (TypedVerilog.BlockingAssign typed_lhs typed_rhs);
   tc_stmt Γ (Verilog.NonBlockingAssign lhs rhs) :=
     typed_lhs <- tc_lvalue Γ lhs ;;
-    typed_rhs <- tc_expr (Some (expr_type typed_lhs)) Γ rhs ;;
+    typed_rhs <- tc_expr (Some (TypedVerilog.expr_type typed_lhs)) Γ rhs ;;
     ret (TypedVerilog.NonBlockingAssign typed_lhs typed_rhs);
   tc_stmt Γ (Verilog.If condition trueBranch falseBranch) :=
     typed_condition <- tc_expr None Γ condition ;;
